Foundation/Modal/Logic/WellKnown.lean
@@ -2,6 +2,7 @@ import Foundation.Modal.Kripke.Hilbert.GL.MDP
 import Foundation.Modal.Kripke.Hilbert.Grz.Completeness
 import Foundation.Modal.Kripke.Hilbert.K4
 import Foundation.Modal.Kripke.Hilbert.K45
+import Foundation.Modal.Kripke.Hilbert.K4Point1
 import Foundation.Modal.Kripke.Hilbert.K4Point2
 import Foundation.Modal.Kripke.Hilbert.K4Point3
 import Foundation.Modal.Kripke.Hilbert.K5
@@ -15,16 +16,20 @@ import Foundation.Modal.Kripke.Hilbert.KD5
 import Foundation.Modal.Kripke.Hilbert.KDB
 import Foundation.Modal.Kripke.Hilbert.KT
 import Foundation.Modal.Kripke.Hilbert.KTB
+import Foundation.Modal.Kripke.Hilbert.KTc
 import Foundation.Modal.Kripke.Hilbert.S4
+import Foundation.Modal.Kripke.Hilbert.S4Point1
 import Foundation.Modal.Kripke.Hilbert.S4Point2
 import Foundation.Modal.Kripke.Hilbert.S4Point3
 import Foundation.Modal.Kripke.Hilbert.GrzPoint2
 import Foundation.Modal.Kripke.Hilbert.GrzPoint3
 import Foundation.Modal.Kripke.Hilbert.GLPoint3
+import Foundation.Modal.Kripke.Hilbert.S4Dot1
+import Foundation.Modal.Kripke.Hilbert.S4Dot2
+import Foundation.Modal.Kripke.Hilbert.S4Dot3
 import Foundation.Modal.Kripke.Hilbert.S5
 import Foundation.Modal.Kripke.Hilbert.Triv
 import Foundation.Modal.Kripke.Hilbert.Ver
-import Foundation.Modal.Kripke.Hilbert.KTc
 import Foundation.Modal.Hilbert.S5Grz
 import Foundation.Modal.Logic.Basic
 import Foundation.Modal.Entailment.KT
@@ -52,6 +57,9 @@ protected abbrev K4Point3 : Logic := Hilbert.K4Point3.logic
 lemma K4Point3.eq_TransitiveWeakConnectedKripkeFrameClass_Logic : Logic.K4Point3 = Kripke.FrameClass.trans_weakConnected.logic
   := eq_Hilbert_Logic_KripkeFrameClass_Logic
 
+protected abbrev K4Dot1 : Logic := Hilbert.K4Dot1.logic
+lemma K4Dot1.eq_TransitiveMcKinseyanKripkeFrameClass_Logic : Logic.K4Dot1 = Kripke.TransitiveMcKinseyanFrameClass.logic
+  := eq_Hilbert_Logic_KripkeFrameClass_Logic
 
 protected abbrev K45 : Logic := Hilbert.K45.logic
 lemma K45.eq_TransitiveEuclideanKripkeFrameClass_Logic : Logic.K45 = Kripke.FrameClass.trans_eucl.logic
@@ -117,6 +125,9 @@ protected abbrev S4 : Logic := Hilbert.S4.logic
 lemma S4.eq_ReflexiveTransitiveKripkeFrameClass_Logic : Logic.S4 = Kripke.FrameClass.preorder.logic
   := eq_Hilbert_Logic_KripkeFrameClass_Logic
 
+protected abbrev S4Dot1 : Logic := Hilbert.S4Dot1.logic
+lemma S4Dot1.eq_ReflexiveTransitiveMcKinseyanKripkeFrameClass_Logic : Logic.S4Dot1 = Kripke.ReflexiveTransitiveMcKinseyanFrameClass.logic
+  := eq_Hilbert_Logic_KripkeFrameClass_Logic
 
 protected abbrev S4Point2 : Logic := Hilbert.S4Point2.logic
 lemma S4Point2.eq_ReflexiveTransitiveConfluentKripkeFrameClass_Logic : Logic.S4Point2 = Kripke.FrameClass.confluent_preorder.logic
