Foundation/Modal/Kripke/AxiomM.lean
@@ -1,0 +1,147 @@
+
+import Foundation.Modal.Kripke.Basic
+import Foundation.Modal.Kripke.Hilbert.Geach
+
+section
+
+variable {α : Type u} (rel : α → α → Prop)
+
+def McKinseyan := ∀ x, ∃ y, rel x y ∧ (∀ z, rel y z → y = z)
+
+end
+
+
+namespace LO.Modal
+
+open Formula.Kripke
+
+namespace Kripke
+
+variable {F : Kripke.Frame}
+
+private lemma not_PseudoMcKinseyan_of_validate_M (h : ¬F ⊧ (Axioms.M (.atom 0))) :
+  ∃ x : F.World, ∀ y, x ≺ y → (∃ z w, (y ≺ z ∧ y ≺ w ∧ z ≠ w))
+  := by
+    obtain ⟨V, x, hx⟩ := ValidOnFrame.exists_valuation_world_of_not h;
+    have := Satisfies.imp_def₂.not.mp hx;
+    push_neg at this;
+    obtain ⟨h₁, h₂⟩ := this;
+    use x;
+    intro y Rxy;
+    obtain ⟨z, Ryz, hz⟩ := Satisfies.dia_def.mp $ h₁ _ Rxy;
+    obtain ⟨w, Ryw, hw⟩ := by
+      have := Satisfies.dia_def.not.mp h₂;
+      push_neg at this;
+      have := Satisfies.box_def.not.mp $ this y Rxy;
+      push_neg at this;
+      exact this;
+    have : z ≠ w := by
+      intro h;
+      subst h;
+      contradiction;
+    use z, w;
+
+private lemma not_McKinseyan_of_notPseudoMcKinseyan
+  (hMc : ∃ x : F.World, ∀ y, x ≺ y → (∃ z w, (y ≺ z ∧ y ≺ w ∧ z ≠ w)))
+  : ¬McKinseyan F.Rel := by
+  unfold McKinseyan;
+  push_neg;
+  obtain ⟨x, h⟩ := hMc;
+  use x;
+  intro y Rxy;
+  obtain ⟨u, v, Ryu, Ryv, huv⟩ := h y Rxy;
+  by_cases hyu : y = u;
+  . subst hyu;
+    use v;
+  . use u;
+
+lemma notMcKinseyan_of_not_validate_M (h : ¬F ⊧ (Axioms.M (.atom 0))) : ¬McKinseyan F.Rel :=
+  not_McKinseyan_of_notPseudoMcKinseyan $ not_PseudoMcKinseyan_of_validate_M h
+
+lemma mcKinseyan_of_validate_M_trans : McKinseyan F → F ⊧ (Axioms.M (.atom 0)) := by
+  contrapose;
+  exact notMcKinseyan_of_not_validate_M;
+
+lemma validate_M_of_mckinseyan_trans (hTrans : Transitive F) : F ⊧ (Axioms.M (.atom 0)) → McKinseyan F := by
+  contrapose;
+  intro hMc;
+  unfold McKinseyan at hMc;
+  push_neg at hMc;
+  obtain ⟨x, h⟩ := hMc;
+  by_cases hDead : ∀ y, ¬x ≺ y;
+  . apply ValidOnFrame.not_of_exists_valuation_world;
+    use (λ _ _ => True), x;
+    suffices (∀ y, x ≺ y → ∃ x, y ≺ x) ∧ ∀ y, ¬x ≺ y by
+      simpa [Satisfies];
+    constructor;
+    . intro y Rxy;
+      have := hDead y Rxy;
+      contradiction;
+    . assumption;
+  . push_neg at hDead;
+    obtain ⟨y, Rxy⟩ := hDead;
+    apply ValidOnFrame.not_of_exists_valuation_world;
+    use (λ z _ =>
+      x ≺ z ∧ ∀ u, x ≺ u → ∃ v, (v ≠ z ∧ u ≺ z ∧ u ≺ v)
+    ), x;
+    apply Satisfies.imp_def₂.not.mpr;
+    push_neg;
+
+    constructor;
+    . apply Satisfies.box_def.mpr;
+      intro w Rxw;
+      apply Satisfies.dia_def.mpr;
+      obtain ⟨z, Rwz, hwz⟩ := h w Rxw;
+      use z;
+      constructor;
+      . assumption;
+      . simp [Semantics.Realize, Satisfies];
+        constructor;
+        . exact hTrans Rxw Rwz;
+        . intro u Rxu;
+          use w;
+          refine ⟨?_, ?_, ?_⟩;
+          . tauto;
+          . sorry
+          . sorry;
+    . apply Satisfies.dia_def.not.mpr
+      push_neg;
+      intro z Rxz;
+      apply Satisfies.box_def.not.mpr;
+      push_neg;
+      obtain ⟨w, Rzw, hzw⟩ := h z Rxz;
+      use w;
+      constructor;
+      . assumption;
+      . simp [Semantics.Realize, Satisfies];
+        intro Rxw;
+        use z;
+        constructor;
+        . assumption;
+        . intro v hvw _;
+          sorry;
+
+abbrev TransitiveMcKinseyanFrameClass : FrameClass := { F | Transitive F ∧ McKinseyan F }
+
+instance TransitiveMcKinseyanFrameClass.DefinedByFourAndM : TransitiveMcKinseyanFrameClass.DefinedBy {Axioms.Four (.atom 0), Axioms.M (.atom 0)} := ⟨by
+  simp only [Set.mem_setOf_eq, Set.mem_insert_iff, Set.mem_singleton_iff, ValidOnFrame.models_iff, forall_eq_or_imp, forall_eq];
+  intro F;
+  constructor;
+  . rintro ⟨hT, hM⟩;
+    refine ⟨?_, ?_⟩;
+    . exact iff_transitive_validate_AxiomFour.mp hT;
+    . exact mcKinseyan_of_validate_M_trans hM;
+  . rintro ⟨hFour, hM⟩;
+    have := iff_transitive_validate_AxiomFour.mpr hFour;
+    constructor;
+    . assumption;
+    . exact validate_M_of_mckinseyan_trans this hM;
+⟩
+
+instance : Kripke.TransitiveMcKinseyanFrameClass.IsNonempty := by
+  use ⟨Unit, λ _ _ => True⟩;
+  simp [Transitive, McKinseyan];
+
+end Kripke
+
+end LO.Modal
