Foundation/Modal/Logic/Sublogic/K4.lean
@@ -6,6 +6,18 @@ open Formula
 open Entailment
 open Kripke
 
+instance : ProperSublogic Logic.K4 Logic.K4Dot1 := ⟨by
+  constructor;
+  . exact Hilbert.weakerThan_of_dominate_axioms (by simp) |>.subset;
+  . suffices ∃ φ, Hilbert.K4Dot1 ⊢! φ ∧ ¬TransitiveFrameClass ⊧ φ by simpa [K4.eq_TransitiveKripkeFrameClass_Logic];
+    use (Axioms.M (.atom 0));
+    constructor;
+    . exact axiomM!;
+    . apply Formula.Kripke.ValidOnFrameClass.not_of_exists_model_world;
+      use ⟨⟨Fin 1, λ x y => False⟩, λ w _ => False⟩, 0;
+      simp [Transitive, Semantics.Realize, Satisfies];
+⟩
+
 instance : ProperSublogic Logic.K4 Logic.K4Point2 := ⟨by
   constructor;
   . exact Hilbert.weakerThan_of_dominate_axioms (by simp) |>.subset;
